rocq-skylabs-brick/tests/cpp_prog_scopes.t/run.t
@@ -1,4 +1,0 @@
-  $ . ../setup-project.sh
-
-Compiling the Coq test file.
-  $ dune build 2>&1
